\documentclass[12pt]{article}

\usepackage{amsmath}
\usepackage{amssymb}
\usepackage{textcomp}
\usepackage{mathpartir}

% Rules from Chapter I in https://arxiv.org/pdf/2212.11082.pdf 

\renewcommand{\.}{\hskip 0.7pt}
\renewcommand{\d}{\;\vdash\,}
\renewcommand{\r}{\!\.\rightarrow\!}
\DeclareMathOperator{\type}{\,type}
\DeclareMathOperator{\id}{id}
\DeclareMathOperator{\comp}{comp}
\newcommand{\N}{\mathbb{N}}
\DeclareMathOperator{\s}{succ}
\DeclareMathOperator{\ind}{ind}
\DeclareMathOperator{\add}{add}
\DeclareMathOperator{\addz}{add-zero}
\DeclareMathOperator{\adds}{add-succ}

\begin{document}

%MLTT rule:
%$$\inferrule
%{\Gamma \d a : A \\ \Gamma \d f : A \r B}
%{\Gamma \d f(a) : B}
%$$
%
%MLTT rule:
%$$\inferrule
%{\Gamma \d a : A}
%{\Gamma,\, x:A \d (a = x) \type}
%$$

\section{Inference rules}

\subsection{Formation of contexts, types, and their elements}

MLTT rule:
$$\inferrule
{\Gamma,\, x\!:\!A \d B(x) \type}
{\Gamma \d A \type}
$$
MLTT rule:
$$\inferrule
{\Gamma \d A \equiv B \type}
{\Gamma \d A \type}
$$
MLTT rule:
$$\inferrule
{\Gamma \d A \equiv B \type}
{\Gamma \d B \type}
$$
MLTT rule:
$$\inferrule
{\Gamma \d a\!:\!A}
{\Gamma \d A \type}
$$
MLTT rule:
$$\inferrule
{\Gamma \d a \equiv b\.\!:\!A}
{\Gamma \d a\!:\!A}
$$
MLTT rule:
$$\inferrule
{\Gamma \d a \equiv b\.\!:\!A}
{\Gamma \d b\.\!:\!A}
$$

\subsection{Judgemental equality is an equivalence relation}

MLTT rule:% (reflexivity on types):
$$\inferrule
{\Gamma \d A \type}
{\Gamma \d A \equiv A \type}
$$
MLTT rule:% (symmetry on types):
$$\inferrule
{\Gamma \d A \equiv B \type}
{\Gamma \d B \equiv A \type}
$$
MLTT rule:% (transitivity on types):
$$\inferrule
{\Gamma \d A \equiv B \type \\ \Gamma \d B \equiv C \type}
{\Gamma \d A \equiv C \type}
$$
MLTT rule:% (reflexivity on elements):
$$\inferrule
{\Gamma \d a\!:\!A}
{\Gamma \d a \equiv a\!:\!A}
$$
MLTT rule:% (symmetry on elements):
$$\inferrule
{\Gamma \d a \equiv b\.\!:\!A}
{\Gamma \d b \equiv a\!:\!A}
$$
MLTT rule:% (transitivity on elements):
$$\inferrule
{\Gamma \d a \equiv b\.\!:\!A \\ \Gamma \d b \equiv c\.\!:\!A}
{\Gamma \d a \equiv c\.\!:\!A}
$$

\subsection{Variable conversion}

MLTT rule:
$$\inferrule
{\Gamma \d A \equiv A' \type \\ \Gamma,\, x\!:\!A,\, \Delta \d B(x) \type}
{\Gamma,\, x\!:\!A',\, \Delta \d B(x) \type}
$$
MLTT rule:
$$\inferrule
{\Gamma \d A \equiv A' \type \\ \Gamma,\, x\!:\!A,\, \Delta \d \mathcal{J}}
{\Gamma,\, x\!:\!A',\, \Delta \d \mathcal{J}}
$$
Derived rule:
$$\inferrule
{\Gamma \d A \equiv A' \type \\ \Gamma \d a\!:\!A}
{\Gamma \d a\!:\!A'}
$$

\subsection{Substitution}

Metasyntactic notation (used in many places):
$$t[a/x] := t \textup{ with all occurences of } x \textup{ replaced by } a$$
MLTT rule:
$$\inferrule
{\Gamma \d a\!:\!A \\ \Gamma,\, x\!:\!A,\, \Delta \d \mathcal{J}}
{\Gamma,\, \Delta[a/x] \d \mathcal{J}[a/x]}
\;S
$$
MLTT rule:
$$\inferrule
{\Gamma \d a \equiv a'\!:\!A \\ \Gamma,\, x\!:\!A,\, \Delta \d B \type}
{\Gamma,\, \Delta[a/x] \d B[a/x] \equiv B[a'\.\!/x] \type}
$$
MLTT rule:
$$\inferrule
{\Gamma \d a \equiv a'\!:\!A \\ \Gamma,\, x\!:\!A,\, \Delta \d b\.\!:\!B}
{\Gamma,\, \Delta[a/x] \d b[a/x] \equiv b[a'\.\!/x] : B[a/x]}
$$

\subsection{Weakening}

MLTT rule:
$$\inferrule
{\Gamma \d A \type \\ \Gamma,\, \Delta \d \mathcal{J}}
{\Gamma,\, x\!:\!A,\, \Delta \d \mathcal{J}}
\;W
$$
MLTT rule:
$$\inferrule
{\Gamma \d A \type \\ \Gamma \d B \type}
{\Gamma,\, x\!:\!A \d B \type}
\;W
$$

\subsection{Generic elements}

MLTT rule:% (variable):
$$\inferrule
{\Gamma \d A \type}
{\Gamma,\, x\!:\!A \d x\!:\!A}
\;\delta
$$

\subsection{Manipulating variables}

Derived rule:
$$\inferrule
{\Gamma,\, x\!:\!A,\, \Delta \d \mathcal{J}}
{\Gamma,\, x'\!:\!A,\, \Delta[x'\.\!/x] \d \mathcal{J}[x'\.\!/x]}
\;x'/x
$$
Derived rule:
$$\inferrule
{\Gamma \d B \type \\ \Gamma,\, x\!:\!A,\, y\!:\!B,\, \Delta \d \mathcal{J}}
{\Gamma,\, y\!:\!B,\, x\!:\!A,\, \Delta \d \mathcal{J}}
$$

\section{$\Pi$ types}

\subsection{Dependent functions}

\subsubsection{$\Pi$ formation}

MLTT rule:
$$\inferrule
{\Gamma,\, x\!:\!A \d B(x) \type}
{\Gamma \d \Pi_{(x:A)} B(x) \type}
\;\Pi
$$
MLTT rule:
$$\inferrule
{\Gamma \d A \equiv A' \type \\ \Gamma,\, x\!:\!A \d B(x) \equiv B'(x) \type}
{\Gamma \d \Pi_{(x:A)} B(x) \equiv \Pi_{(x:A')} B'(x) \type}
\;\Pi\textup{-eq}
$$

\subsubsection{$\Pi$ introduction}

MLTT rule:
$$\inferrule
{\Gamma,\, x\!:\!A \d b(x) : B(x)}
{\Gamma \d \lambda x \..\. b(x) : \Pi_{(x:A)} B(x)}
\;\lambda
$$
MLTT rule:
$$\inferrule
{\Gamma,\, x\!:\!A \d b(x) \equiv b'(x) : B(x)}
{\Gamma \d \lambda x \..\. b(x) \,\equiv\, \lambda x \..\. b'(x) : \Pi_{(x:A)} B(x)}
\;\lambda\textup{-eq}
$$

\subsubsection{$\Pi$ elimination}

MLTT rule:
$$\inferrule
{\Gamma \d f : \Pi_{(x:A)} B(x)}
{\Gamma,\, x\!:\!A \d f(x) : B(x)}
\;\textup{ev}
$$
MLTT rule:
$$\inferrule
{\Gamma \d f \equiv f' \!\.: \Pi_{(x:A)} B(x)}
{\Gamma,\, x\!:\!A \d f(x) \equiv f'(x) : B(x)}
\;\textup{ev-eq}
$$

\subsubsection{$\Pi$ computation}

MLTT rule:
$$\inferrule
{\Gamma,\, x\!:\!A \d b(x) : B(x)}
{\Gamma,\, x\!:\!A \d (\lambda y . b(y))(x) \.\equiv\. b(x) : B(x)}
\;\beta
$$
MLTT rule:
$$\inferrule
{\Gamma \d f : \Pi_{(x:A)} B(x)}
{\Gamma \d \lambda x \..\. f(x) \,\equiv\, f : \Pi_{(x:A)} B(x)}
\;\eta
$$

\subsection{Ordinary functions}

\subsubsection{Basic}

%$$\inferrule
%{\Gamma \d A \type \\ \Gamma \d B \type}
%{\Gamma \d A \r B \coloneq \Pi_{(x:A)} B \type}
%$$
MLTT rule:
$$\inferrule
{\Gamma \d A \type \\ \Gamma \d B \type}
{\Gamma \d A \r B \type}
\;\rightarrow
$$
MLTT rule:
$$\inferrule
{\Gamma \d A \type \\ \Gamma \d B \type}
{\Gamma \d A \r B \.\equiv\. \Pi_{(x:A)} B \type}
$$
Derived rule:
$$\inferrule
{\Gamma \d B \type \\ \Gamma,\, x\!:\!A \d b(x) : B(x)}
{\Gamma \d \lambda x \..\. b(x) : A \r B}
\;\lambda
$$
Derived rule:
$$\inferrule
{\Gamma \d f : A \r B}
{\Gamma,\, x\!:\!A \d f(x) : B}
\;\textup{ev}
$$
Derived rule:
$$\inferrule
{\Gamma \d B \type \\ \Gamma,\, x\!:\!A \d b(x) : B}
{\Gamma,\, x\!:\!A \d (\lambda y . b(y))(x) \.\equiv\. b(x) : B}
\;\beta
$$
Derived rule:
$$\inferrule
{\Gamma \d f : A \r B}
{\Gamma \d \lambda x \..\. f(x) \,\equiv\, f : A \r B}
\;\eta
$$

\subsubsection{Identity function}

MLTT rule:
$$\inferrule
{\Gamma \d A \type}
{\Gamma \d \id_A : A \r A}
$$
MLTT rule:
$$\inferrule
{\Gamma \d A \type \\ \Gamma \d B \type}
{\Gamma \d \id_A \.\equiv\. \lambda x .\. x : A \r A}
$$

\subsubsection{Composition}

MLTT rule:
$$\inferrule
{\Gamma \d A \type \\ \Gamma \d B \type \\ \Gamma \d C \type}
{\Gamma \d \comp : (B \r C) \r (A \r B) \r (A \r C)}
$$
MLTT rule:
$$\inferrule
{\Gamma \d A \type \\ \Gamma \d B \type \\ \Gamma \d C \type}
{\Gamma \d \comp \equiv \lambda g .\. \lambda f .\. \lambda x .\. g(f(x)) : (B \r C) \r (A \r B) \r (A \r C)}
$$
Remark:
$$g \circ f \equiv \comp(g,f) \equiv \lambda x.\. g(f(x)) $$
Derived rule:
$$\inferrule
{\Gamma \d f : A \r B \\ \Gamma \d g : B \r C \\ \Gamma \d h : C \!\rightarrow\! D}
{\Gamma \d (h \circ g) \circ f \,\equiv\, h \circ (g \circ f) : A \r D}
$$

\section{The natural numbers}

\subsection{Basic}

MLTT rule:
$$\inferrule
{~}
{\d \N \type}
\;\N\textup{-form}
$$
MLTT rule:
$$\inferrule
{~}
{\d 0_\N : \N}
$$
MLTT rule:
$$\inferrule
{~}
{\d \s_\N : \N}
$$

\subsection{Induction principle}

Metasyntactic shortcut (only for this document):
$$\textup{\textcircledP} \quad := \quad \Gamma,\, n\!\.:\!\.\N \d P(n) \type$$
MLTT rule:
$$\inferrule
{\textup{\textcircledP} \\ \Gamma \d p_0 : P(0_\N) \\ \Gamma \d p_S : \Pi_{(n:\N)} \left( P(n) \r P(\s_\N(n)) \right) }
{\Gamma \d \ind_\N(p_0, p_S) : \Pi_{(n:\N)} P(n)}
\;\N\textup{-ind}
$$
%MLTT rule:
%$$\inferrule
%{\Gamma,\, n\!\.:\!\.\N \d P(n) \type}
%{\Gamma \d \ind_\N : P(0_\N) \r \left( \Pi_{(n:\N)} \left( P(n) \r P(\s_\N(n)) \right) \right) \r \Pi_{(n:\N)} P(n)}
%\;\N\textup{-ind}
%$$
MLTT rule:
$$\inferrule
{\textup{\textcircledP} \\ \Gamma \d p_0 : P(0_\N) \\ \Gamma \d p_S : \Pi_{(n:\N)} \left( P(n) \r P(\s_\N(n)) \right) }
{\Gamma \d \ind_\N(p_0, p_S, 0_\N) \equiv p_0 : P(0_\N)}
$$
MLTT rule:
$$\inferrule
{\textup{\textcircledP} \\ \Gamma \d p_0 : P(0_\N) \\ \Gamma \d p_S : \Pi_{(n:\N)} \left( P(n) \r P(\s_\N(n)) \right) }
{\Gamma,\, n\!\.:\!\.\N \d \ind_\N(p_0, p_S, \s_\N(n)) \equiv p_S(n, \ind_\N(p_0, p_S, n)) : P(\s_\N(n))}
$$
%For example (I just derived):
%$$\inferrule
%{\circledast \\ \Gamma \d p_0 : P(0_\N) \\ \Gamma \d p_S : \Pi_{(n:\N)} \left( P(n) \r P(\s_\N(n)) \right) }
%{\Gamma \d \ind_\N(p_0, p_S, \s_\N(0_\N)) \equiv p_S(0_\N, p_0) : P(\s_\N(0_\N))}
%$$

\newpage
\subsection{Addition}

MLTT rule:
$$\inferrule
{~}
{m : \N \d \addz_\N(m) : \N}
$$
MLTT rule:
$$\inferrule
{~}
{m : \N \d \addz_\N(m) \equiv m : \N}
$$
MLTT rule:
$$\inferrule
{~}
{m : \N \d \adds_\N(m) : \N \r \N \r \N}
$$
MLTT rule:
$$\inferrule
{~}
{m : \N \d \adds_\N(m) \equiv \lambda n \.. \s_\N : \N \r \N \r \N}
$$
MLTT rule:
$$\inferrule
{~}
{m : \N \d \add_\N(m) : \N \r \N}
$$
MLTT rule:
$$\inferrule
{~}
{m : \N \d \add_\N(m) \equiv \ind_\N(\addz_\N(m), \adds_\N(m)) : \N \r \N}
$$
Remark:
$$m + 0_\N \equiv \add_\N(m, 0_\N) \equiv m$$
Remark:
$$m + \s_\N(n) \equiv \add_\N(m, \s_\N(n)) \equiv \s_\N(m+n)$$

\end{document}